Superposition_Calculus/First_Order_Type_System.thy
@@ -1,0 +1,170 @@
+theory First_Order_Type_System
+  imports First_Order_Clause
+begin
+
+inductive has_type for \<F> \<V> where
+  Var: "\<V> x = \<tau> \<Longrightarrow> has_type \<F> \<V> (Var x) \<tau>" |
+  Fun: "\<F> f = (\<tau>s, \<tau>) \<Longrightarrow> 
+    list_all2 (has_type \<F> \<V>) ts \<tau>s \<Longrightarrow>
+    has_type \<F> \<V> (Fun f ts) \<tau>"
+
+lemma right_unique_has_type: "right_unique (has_type \<F> \<V>)"
+proof (rule right_uniqueI)
+  fix t \<tau>\<^sub>1 \<tau>\<^sub>2
+  assume "has_type \<F> \<V> t \<tau>\<^sub>1" and "has_type \<F> \<V> t \<tau>\<^sub>2"
+  thus "\<tau>\<^sub>1 = \<tau>\<^sub>2"
+    by (auto elim!: has_type.cases)
+qed
+
+definition well_typed_atm where
+  "well_typed_atm \<F> \<V> A \<longleftrightarrow> (\<exists>\<tau>. \<forall>t \<in> set_uprod A. has_type \<F> \<V> t \<tau>)"
+
+definition well_typed_lit where
+  "well_typed_lit \<F> \<V> L \<longleftrightarrow> well_typed_atm \<F> \<V> (atm_of L)"
+
+definition well_typed_cls where
+  "well_typed_cls \<F> \<V> C \<longleftrightarrow> (\<forall>L \<in># C. well_typed_lit \<F> \<V> L)"
+
+definition well_typed_cls_set where
+  "well_typed_cls_set \<F> \<V> N \<longleftrightarrow> (\<forall>C \<in> N. well_typed_cls \<F> \<V> C)"
+
+definition well_typed_subst where
+  "well_typed_subst \<F> \<V> \<sigma> \<longleftrightarrow> (\<forall>x. has_type \<F> \<V> (\<sigma> x) (\<V> x))"
+
+lemma well_typed_cls_add_mset: 
+  "well_typed_cls \<F> \<V> (add_mset L C) \<longleftrightarrow> well_typed_lit \<F> \<V> L \<and> well_typed_cls \<F> \<V> C"
+  by (simp add: well_typed_cls_def)
+
+lemma well_typed_cls_plus: 
+  "well_typed_cls \<F> \<V> (C + D) \<longleftrightarrow> well_typed_cls \<F> \<V> C \<and> well_typed_cls \<F> \<V> D"
+  by (auto simp: well_typed_cls_def)
+
+lemma well_typed_subst_term: 
+  assumes well_typed_subst: "well_typed_subst \<F> \<V> \<sigma>"
+  shows "has_type \<F> \<V> (t \<cdot>t \<sigma>) \<tau> \<longleftrightarrow> has_type \<F> \<V> t \<tau>"
+proof(rule iffI)
+  assume "has_type \<F> \<V> (t \<cdot>t \<sigma>) \<tau>"
+  thus "has_type \<F> \<V> t \<tau>"
+  proof(induction "t \<cdot>t \<sigma>" \<tau>  arbitrary: t rule: has_type.induct)
+    case (Var x \<tau>)
+    then obtain x' where t: "t = Var x'"
+      by (metis subst_apply_eq_Var)
+
+    have "has_type \<F> \<V> t (\<V> x')"
+      unfolding t 
+      by (simp add: has_type.Var)
+
+    have "has_type \<F> \<V> t (\<V> x)"
+      using Var well_typed_subst
+      unfolding t well_typed_subst_def
+      by (metis eval_term.simps(1) has_type.Var right_uniqueD right_unique_has_type)
+
+    then have \<V>_x': "\<tau> = \<V> x'"
+      using Var well_typed_subst
+      unfolding well_typed_subst_def  t
+      by (metis has_type.Var right_uniqueD right_unique_has_type t)
+
+    show ?case 
+      unfolding t \<V>_x'
+      by (simp add: has_type.Var)
+  next
+    case (Fun f \<tau>s \<tau> ts)
+    show ?case 
+    proof(cases t)
+      case (Var x)
+      from Fun show ?thesis
+        using  well_typed_subst 
+        unfolding well_typed_subst_def Var
+        by (metis (no_types, opaque_lifting) eval_term.simps(1) has_type.simps prod.sel(2) 
+              term.distinct(1) term.inject(2))
+    next
+      case Fun\<^sub>t: Fun
+      with Fun show ?thesis
+        by (simp add: has_type.simps list.rel_map(1) list_all2_mono)
+    qed
+  qed
+next
+  assume "has_type \<F> \<V> t \<tau>"
+  thus "has_type \<F> \<V> (t \<cdot>t \<sigma>) \<tau>"
+  proof(induction t \<tau>  rule: has_type.induct)
+    case Var\<^sub>t: (Var x \<tau>)
+    then show ?case
+    proof(cases "Var x \<cdot>t \<sigma>")
+      case Var
+      then show ?thesis
+        using well_typed_subst
+        unfolding well_typed_subst_def
+        by (metis Var\<^sub>t.hyps eval_term.simps(1))        
+    next
+      case Fun
+      then show ?thesis
+        using well_typed_subst
+        unfolding well_typed_subst_def
+        by (metis Var\<^sub>t.hyps eval_term.simps(1))    
+    qed
+  next
+    case (Fun f \<tau>s \<tau> ts)
+    then show ?case
+      using assms list_all2_mono
+      unfolding well_typed_subst_def
+      by (smt (verit, ccfv_SIG) eval_term.simps(2) has_type.simps list.rel_map(1))
+  qed
+qed
+
+lemma well_typed_subst_atom: 
+  assumes well_typed_subst: "well_typed_subst \<F> \<V> \<sigma>"
+  shows "well_typed_atm \<F> \<V> (a \<cdot>a \<sigma>) \<longleftrightarrow> well_typed_atm \<F> \<V> a"
+  using well_typed_subst_term[OF well_typed_subst]
+  unfolding well_typed_atm_def subst_atom_def
+  by(cases a) simp
+
+lemma well_typed_subst_literal: 
+  assumes well_typed_subst: "well_typed_subst \<F> \<V> \<sigma>"
+  shows "well_typed_lit \<F> \<V> (l \<cdot>l \<sigma>) \<longleftrightarrow> well_typed_lit \<F> \<V> l"
+  using well_typed_subst_atom[OF well_typed_subst]
+  unfolding well_typed_lit_def subst_literal_def
+  by(cases l) auto
+
+lemma well_typed_subst_clause: 
+  assumes well_typed_subst: "well_typed_subst \<F> \<V> \<sigma>"
+  shows "well_typed_cls \<F> \<V> (c \<cdot> \<sigma>) \<longleftrightarrow> well_typed_cls \<F> \<V> c"
+  using well_typed_subst_literal[OF well_typed_subst]
+  unfolding well_typed_cls_def subst_clause_def
+  by blast
+
+lemma ctxt_apply_term_preserves_typing:
+  assumes
+    \<kappa>_type: "has_type \<F> \<V> \<kappa>\<langle>t\<rangle> \<tau>\<^sub>1" and
+    t_type: "has_type \<F> \<V> t \<tau>\<^sub>2" and
+    t'_type: "has_type \<F> \<V> t' \<tau>\<^sub>2"
+  shows "has_type \<F> \<V> \<kappa>\<langle>t'\<rangle> \<tau>\<^sub>1"
+  using \<kappa>_type
+proof (induction \<kappa> arbitrary: \<tau>\<^sub>1)
+  case Hole
+  then show ?case
+    using t_type t'_type
+    using right_unique_has_type[of \<F>, THEN right_uniqueD]
+    by auto
+next
+  case (More f ss1 \<kappa> ss2)
+  have "has_type \<F> \<V> (Fun f (ss1 @ \<kappa>\<langle>t\<rangle> # ss2)) \<tau>\<^sub>1"
+    using More.prems by simp
+  hence "has_type \<F> \<V> (Fun f (ss1 @ \<kappa>\<langle>t'\<rangle> # ss2)) \<tau>\<^sub>1"
+  proof (cases \<F> \<V> "Fun f (ss1 @ \<kappa>\<langle>t\<rangle> # ss2)" \<tau>\<^sub>1 rule: has_type.cases)
+    case (Fun \<tau>s)
+    show ?thesis
+    proof (rule has_type.Fun)
+      show "\<F> f = (\<tau>s, \<tau>\<^sub>1)"
+        using \<open>\<F> f = (\<tau>s, \<tau>\<^sub>1)\<close> .
+    next
+      show "list_all2 (has_type \<F> \<V>) (ss1 @ \<kappa>\<langle>t'\<rangle> # ss2) \<tau>s"
+        using \<open>list_all2 (has_type \<F> \<V>) (ss1 @ \<kappa>\<langle>t\<rangle> # ss2) \<tau>s\<close>
+        using More.IH
+        by (smt (verit, del_insts) list_all2_Cons1 list_all2_append1 list_all2_lengthD)
+    qed
+  qed
+  thus ?case
+    by simp
+qed
+
+end
